13AssemblyCode/Assemble.thy
@@ -3,79 +3,106 @@ theory Assemble
 begin
 
 primrec assemble_op_len :: "byte_code \<Rightarrow> nat" where
-  "assemble_op_len (BLookup x) = 6 + 2 * x"
-| "assemble_op_len (BPushCon k) = 6"
-| "assemble_op_len (BPushLam pc) = 9"
-| "assemble_op_len BApply = 17"
-| "assemble_op_len BReturn = 3"
-| "assemble_op_len BJump = 15"
+  "assemble_op_len (BLookup x) = 9 + 2 * x"
+| "assemble_op_len (BPushCon k) = 10"
+| "assemble_op_len (BPushLam pc) = 13"
+| "assemble_op_len BApply = 24"
+| "assemble_op_len BReturn = 5"
+| "assemble_op_len BJump = 22"
 
 primrec assemble_op :: "(nat \<Rightarrow> nat) \<Rightarrow> byte_code \<Rightarrow> assm_code list" where
   "assemble_op mp (BLookup x) = [
     AMov Acc (Con 0),
-    APush Vals (Reg Acc),
-    AGet Env Acc,
+    AAdd Vals 1,
+    APut Vals Vals (Reg Acc),
+    AGet Acc Env Acc,
     ASub Acc 2] @
     concat (replicate x [
-    AGet Env Acc,
+    AGet Acc Env Acc,
     ASub Acc 1]) @ [
-    APush Stk (Reg Acc),
-    APop Stk]"
+    AAdd Stk 1,
+    APut Stk Stk (Reg Acc),
+    AGet Acc Stk Stk,
+    ASub Stk 1]"
 | "assemble_op mp (BPushCon k) = [
     AMov Acc (Con 0),
-    APush Hp (Con 0), 
-    APush Hp (Con k), 
-    APush Hp (Con 1), 
-    APush Vals (Reg Acc), 
+    AAdd Hp 1, 
+    APut Hp Hp (Con 0),
+    AAdd Hp 1,  
+    APut Hp Hp (Con k),
+    AAdd Hp 1,  
+    APut Hp Hp (Con 1), 
+    AAdd Vals 1,
+    APut Vals Vals (Reg Acc),
     AMov Acc (Reg Hp)]"
 | "assemble_op mp (BPushLam pc) = [
+    AAdd Hp 1, 
+    APut Hp Hp (Con (mp pc)), 
     AMov Acc (Con 0),
-    APush Hp (Con (mp pc)), 
-    APush Hp (Reg Acc), 
-    APush Hp (Con 0),
-    AGet Stk Acc, 
+    AAdd Hp 1, 
+    APut Hp Hp (Reg Acc),
+    AAdd Hp 1, 
+    APut Hp Hp (Con 0),
+    AGet Acc Stk Acc, 
     ASub Acc 1,
     AMov Acc (Reg Stk),
-    APush Vals (Reg Acc), 
+    AAdd Vals 1,
+    APut Vals Vals (Reg Acc),
     AMov Acc (Reg Hp)]"
 | "assemble_op mp BApply = [
     AJump,
-    AGet Hp Acc,
+    AGet Acc Hp Acc,
     AAdd Acc 1,
+    AMov Acc2 (Con 0),
     AMov Acc (Reg Acc2),
-    APush Env (Reg Acc),
-    AGet Hp Acc,
+    AAdd Env 1,
+    APut Env Env (Reg Acc),
+    AGet Acc Hp Acc,
     AMov Acc2 (Reg Acc),
     AAdd Acc 1,
-    APop Vals,
-    APush Stk (Reg Acc),
+    AGet Acc Vals Vals,
+    ASub Vals 1,
+    AAdd Stk 1,
+    APut Stk Stk (Reg Acc),
     AAdd Acc 1,
     AMov Acc (Reg Env),
-    APush Stk (Reg Acc),
-    ASub Acc 14,
+    AAdd Stk 1,
+    APut Stk Stk (Reg Acc),
+    ASub Acc 19,
     AMov Acc PC,
-    APush Env (Reg Acc),
-    APop Vals]"
+    AAdd Env 1,
+    APut Env Env (Reg Acc),
+    AGet Acc Vals Vals,
+    ASub Vals 1]"
 | "assemble_op mp BReturn = [
     AJump,
-    APop Stk,
-    APop Stk]"
+    AGet Acc Stk Stk,
+    ASub Stk 1,
+    AGet Acc Stk Stk,
+    ASub Stk 1]"
 | "assemble_op mp BJump = [
     AJump,
-    AGet Hp Acc,
+    AGet Acc Hp Acc,
     AAdd Acc 1,
+    AMov Acc2 (Con 0),
     AMov Acc (Reg Acc2),
-    APush Env (Reg Acc),
-    AGet Hp Acc,
+    AAdd Env 1,
+    APut Env Env (Reg Acc),
+    AGet Acc Hp Acc,
     AMov Acc2 (Reg Acc),
     AAdd Acc 1,
-    APop Vals,
-    APush Stk (Reg Acc),
+    AGet Acc Vals Vals,
+    ASub Vals 1,
+    AAdd Stk 1,
+    APut Stk Stk (Reg Acc),
     AAdd Acc 1,
     AMov Acc (Reg Env),
-    APop Stk,
-    APush Env (Reg Acc),
-    APop Vals]"
+    AGet Acc Stk Stk,
+    ASub Stk 1,
+    AAdd Env 1,
+    APut Env Env (Reg Acc),
+    AGet Acc Vals Vals,
+    ASub Vals 1]"
 
 abbreviation assemble_extend_map :: "(nat \<Rightarrow> nat) \<Rightarrow> nat \<Rightarrow> nat \<Rightarrow> nat \<Rightarrow> nat" where
   "assemble_extend_map mp b lop x \<equiv> (if x < b then mp x else mp x + lop - 1)"
@@ -294,34 +321,35 @@ proof (induction y arbitrary: x)
 qed simp_all
 
 lemma [simp]: "unstr_lookup e a x = Some v \<Longrightarrow> cd ! pc = BLookup y \<Longrightarrow> x \<le> y \<Longrightarrow> 
-  pc < length cd \<Longrightarrow> iter_evala (assemble_code cd) (4 + 2 * x) 
+  pc < length cd \<Longrightarrow> iter_evala (assemble_code cd) (5 + 2 * x) 
     (AS (case_register h e vs sh am bm) (case_register hp ep vp sp a 0) 
-      (4 + 2 * x + assembly_map cd pc)) = Some (AS (case_register h e (vs(vp := v)) sh am bm) 
+      (5 + 2 * x + assembly_map cd pc)) = Some (AS (case_register h e (vs(vp := v)) sh am bm) 
         (case_register hp ep (Suc vp) sp 0 0) (assembly_map cd pc))"
 proof (induction e a x rule: unstr_lookup.induct)
   case (3 e p)
-  moreover from 3 have "assemble_code cd ! (3 + assembly_map cd pc) = ASub Acc 2" by simp
-  moreover from 3 have "assemble_code cd ! (2 + assembly_map cd pc) = AGet Env Acc" 
+  moreover from 3 have "assemble_code cd ! (4 + assembly_map cd pc) = ASub Acc 2" by simp
+  moreover from 3 have "assemble_code cd ! (3 + assembly_map cd pc) = AGet Acc Env Acc" 
+    by simp
+  moreover from 3 have "assemble_code cd ! (2 + assembly_map cd pc) = APut Vals Vals (Reg Acc)" 
     by (simp del: add_2_eq_Suc) 
   ultimately show ?case by (simp add: numeral_def)
 next
   case (4 e p x)
-  hence "assemble_code cd ! (5 + 2 * x + assembly_map cd pc) = ASub Acc (Suc 0)" 
-    by simp
-  moreover from 4 have "assemble_code cd ! (4 + 2 * x + assembly_map cd pc) = AGet Env Acc" 
+  hence "assemble_code cd ! (6 + 2 * x + assembly_map cd pc) = ASub Acc (Suc 0)" by simp
+  moreover from 4 have "assemble_code cd ! (5 + 2 * x + assembly_map cd pc) = AGet Acc Env Acc" 
     by simp
   ultimately have "iter_evala (assemble_code cd) 2
     (AS (case_register h e vs sh am bm) (case_register hp ep vp sp (Suc (Suc p)) 0)
-      (6 + 2 * x + assembly_map cd pc)) = Some (AS (case_register h e vs sh am bm) 
-        (case_register hp ep vp sp (e (Suc p)) 0) (4 + 2 * x + assembly_map cd pc))" 
+      (7 + 2 * x + assembly_map cd pc)) = Some (AS (case_register h e vs sh am bm) 
+        (case_register hp ep vp sp (e (Suc p)) 0) (5 + 2 * x + assembly_map cd pc))" 
     by (simp add: numeral_def)
-  moreover from 4 have "iter_evala (assemble_code cd) (4 + 2 * x) 
+  moreover from 4 have "iter_evala (assemble_code cd) (5 + 2 * x) 
     (AS (case_register h e vs sh am bm) (case_register hp ep vp sp (e (Suc p)) 0) 
-      (4 + 2 * x + assembly_map cd pc)) = Some (AS (case_register h e (vs(vp := v)) sh am bm) 
+      (5 + 2 * x + assembly_map cd pc)) = Some (AS (case_register h e (vs(vp := v)) sh am bm) 
         (case_register hp ep (Suc vp) sp 0 0) (assembly_map cd pc))" by simp 
-  ultimately have "iter_evala (assemble_code cd) (2 + (4 + 2 * x))
+  ultimately have "iter_evala (assemble_code cd) (2 + (5 + 2 * x))
     (AS (case_register h e vs sh am bm) (case_register hp ep vp sp (Suc (Suc p)) 0)
-      (6 + 2 * x + assembly_map cd pc)) = Some (AS (case_register h e (vs(vp := v)) sh am bm)
+      (7 + 2 * x + assembly_map cd pc)) = Some (AS (case_register h e (vs(vp := v)) sh am bm)
         (case_register hp ep (Suc vp) sp 0 0) (assembly_map cd pc))" 
     using iter_evala_combine by blast
   thus ?case by simp
@@ -332,39 +360,48 @@ theorem correcta [simp]: "cd\<^sub>b \<tturnstile> \<Sigma>\<^sub>u \<leadsto>\<
 proof (induction cd\<^sub>b \<Sigma>\<^sub>u \<Sigma>\<^sub>u' rule: evalu.induct)
   case (evu_lookup cd pc x e sh sp y h hp ep vs vp)
   moreover hence "odd sp" by simp
-  moreover from evu_lookup have "assemble_code cd ! (5 + 2 * x + assembly_map cd pc) = APop Stk" 
+  moreover from evu_lookup have "assemble_code cd ! (8 + 2 * x + assembly_map cd pc) = ASub Stk 1" 
     by (simp add: nth_append)
-  moreover from evu_lookup have "assemble_code cd ! (4 + 2 * x + assembly_map cd pc) = 
-    APush Stk (Reg Acc)" by (simp add: nth_append)
-  ultimately have "iter_evala (assemble_code cd) 2 
+  moreover from evu_lookup have "assemble_code cd ! (7 + 2 * x + assembly_map cd pc) = 
+    AGet Acc Stk Stk" by (simp add: nth_append)
+  moreover from evu_lookup have "assemble_code cd ! (6 + 2 * x + assembly_map cd pc) = 
+    APut Stk Stk (Reg Acc)" by (simp add: nth_append)
+  moreover from evu_lookup have "assemble_code cd ! (5 + 2 * x + assembly_map cd pc) = 
+    AAdd Stk 1" by (simp add: nth_append)
+  ultimately have "iter_evala (assemble_code cd) 4 
     (AS (case_register (assm_hp cd h) e vs (assm_stk cd sh) nmem nmem) 
-      (case_register hp ep vp (Suc sp) 0 0) (6 + 2 * x + assembly_map cd pc)) = 
+      (case_register hp ep vp (Suc sp) 0 0) (9 + 2 * x + assembly_map cd pc)) = 
         Some (AS (case_register (assm_hp cd h) e vs (assm_stk cd sh) nmem nmem) 
-          (case_register hp ep vp (Suc sp) (sh sp) 0) (4 + 2 * x + assembly_map cd pc))" 
+          (case_register hp ep vp (Suc sp) (sh sp) 0) (5 + 2 * x + assembly_map cd pc))" 
     by (simp add: numeral_def)
-  moreover from evu_lookup have "iter_evala (assemble_code cd) (4 + 2 * x) 
+  moreover from evu_lookup have "iter_evala (assemble_code cd) (5 + 2 * x) 
     (AS (case_register (assm_hp cd h) e vs (assm_stk cd sh) nmem nmem) 
-      (case_register hp ep vp (Suc sp) (sh sp) 0) (4 + 2 * x + assembly_map cd pc)) = 
+      (case_register hp ep vp (Suc sp) (sh sp) 0) (5 + 2 * x + assembly_map cd pc)) = 
         Some (AS (case_register (assm_hp cd h) e (vs(vp := y)) (assm_stk cd sh) nmem nmem) 
           (case_register hp ep (Suc vp) (Suc sp) 0 0) (assembly_map cd pc))" by simp
-  ultimately have "iter_evala (assemble_code cd) (2 + (4 + 2 * x)) 
+  ultimately have "iter_evala (assemble_code cd) (4 + (5 + 2 * x)) 
     (AS (case_register (assm_hp cd h) e vs (assm_stk cd sh) nmem nmem) 
-      (case_register hp ep vp (Suc sp) 0 0) (6 + 2 * x + assembly_map cd pc)) = 
+      (case_register hp ep vp (Suc sp) 0 0) (9 + 2 * x + assembly_map cd pc)) = 
         Some (AS (case_register (assm_hp cd h) e (vs(vp := y)) (assm_stk cd sh) nmem nmem)
           (case_register hp ep (Suc vp) (Suc sp) 0 0) (assembly_map cd pc))" 
     using iter_evala_combine by blast
   with evu_lookup show ?case by auto
 next
   case (evu_pushcon cd pc k h hp e ep vs vp sh sp)
-  moreover from evu_pushcon have "assemble_code cd ! (5 + assembly_map cd pc) = AMov Acc (Reg Hp)" 
+  moreover from evu_pushcon have "assemble_code cd ! (9 + assembly_map cd pc) = AMov Acc (Reg Hp)" 
     by simp
-  moreover from evu_pushcon have "assemble_code cd ! (4 + assembly_map cd pc) = 
-    APush Vals (Reg Acc)" by simp
-  moreover from evu_pushcon have "assemble_code cd ! (3 + assembly_map cd pc) = APush Hp (Con 1)" 
+  moreover from evu_pushcon have "assemble_code cd ! (8 + assembly_map cd pc) = 
+    APut Vals Vals (Reg Acc)" by simp
+  moreover from evu_pushcon have "assemble_code cd ! (7 + assembly_map cd pc) = AAdd Vals 1" by simp
+  moreover from evu_pushcon have "assemble_code cd ! (6 + assembly_map cd pc) = APut Hp Hp (Con 1)" 
     by simp
-  moreover from evu_pushcon have "assemble_code cd ! (2 + assembly_map cd pc) = APush Hp (Con k)" 
+  moreover from evu_pushcon have "assemble_code cd ! (5 + assembly_map cd pc) = AAdd Hp 1" by simp
+  moreover from evu_pushcon have "assemble_code cd ! (4 + assembly_map cd pc) = APut Hp Hp (Con k)" 
+    by simp
+  moreover from evu_pushcon have "assemble_code cd ! (3 + assembly_map cd pc) = AAdd Hp 1" by simp
+  moreover from evu_pushcon have "assemble_code cd ! (2 + assembly_map cd pc) = APut Hp Hp (Con 0)" 
     by (simp del: add_2_eq_Suc) 
-  ultimately have "iter_evala (assemble_code cd) 6 (AS (case_register (assm_hp cd h) e vs 
+  ultimately have "iter_evala (assemble_code cd) 10 (AS (case_register (assm_hp cd h) e vs 
     (assm_stk cd sh) nmem nmem) (case_register hp ep vp (Suc sp) 0 0) (assembly_map cd (Suc pc))) = 
       Some (AS (case_register (assm_hp cd (h(hp := 1, Suc hp := k, Suc (Suc hp) := 0))) e 
         (vs(vp := hp)) (assm_stk cd sh) nmem nmem) (case_register (3 + hp) ep (Suc vp) (Suc sp) 0 0)
@@ -373,20 +410,26 @@ next
   thus ?case by auto
 next
   case (evu_pushlam cd pc pc' h hp e ep vs vp sh sp)
-  moreover from evu_pushlam have "assemble_code cd ! (8 + assembly_map cd pc) = AMov Acc (Reg Hp)" 
+  moreover from evu_pushlam have "assemble_code cd ! (12 + assembly_map cd pc) = AMov Acc (Reg Hp)" 
     by simp
-  moreover from evu_pushlam have "assemble_code cd ! (7 + assembly_map cd pc) = 
-    APush Vals (Reg Acc)" by simp
-  moreover from evu_pushlam have "assemble_code cd ! (6 + assembly_map cd pc) = AMov Acc (Reg Stk)" 
+  moreover from evu_pushlam have "assemble_code cd ! (11 + assembly_map cd pc) = 
+    APut Vals Vals (Reg Acc)" by simp
+  moreover from evu_pushlam have "assemble_code cd ! (10 + assembly_map cd pc) = AAdd Vals 1" 
     by simp
-  moreover from evu_pushlam have "assemble_code cd ! (5 + assembly_map cd pc) = ASub Acc 1" by simp
-  moreover from evu_pushlam have "assemble_code cd ! (4 + assembly_map cd pc) = AGet Stk Acc" 
+  moreover from evu_pushlam have "assemble_code cd ! (9 + assembly_map cd pc) = AMov Acc (Reg Stk)" 
     by simp
-  moreover from evu_pushlam have "assemble_code cd ! (3 + assembly_map cd pc) = APush Hp (Con 0)" 
+  moreover from evu_pushlam have "assemble_code cd ! (8 + assembly_map cd pc) = ASub Acc 1" by simp
+  moreover from evu_pushlam have "assemble_code cd ! (7 + assembly_map cd pc) = AGet Acc Stk Acc" 
+    by simp
+  moreover from evu_pushlam have "assemble_code cd ! (6 + assembly_map cd pc) = APut Hp Hp (Con 0)" 
     by simp 
-  moreover from evu_pushlam have "assemble_code cd ! (2 + assembly_map cd pc) = APush Hp (Reg Acc)" 
+  moreover from evu_pushlam have "assemble_code cd ! (5 + assembly_map cd pc) = AAdd Hp 1" by simp 
+  moreover from evu_pushlam have "assemble_code cd ! (4 + assembly_map cd pc) =
+    APut Hp Hp (Reg Acc)" by simp
+  moreover from evu_pushlam have "assemble_code cd ! (3 + assembly_map cd pc) = AAdd Hp 1" by simp 
+  moreover from evu_pushlam have "assemble_code cd ! (2 + assembly_map cd pc) = AMov Acc (Con 0)" 
     by (simp del: add_2_eq_Suc) 
-  ultimately have "iter_evala (assemble_code cd) 9 (AS (case_register (assm_hp cd h) e vs 
+  ultimately have "iter_evala (assemble_code cd) 13 (AS (case_register (assm_hp cd h) e vs 
     (assm_stk cd sh) nmem nmem) (case_register hp ep vp (Suc sp) 0 0) (assembly_map cd (Suc pc))) = 
       Some (AS (case_register (assm_hp cd (h(hp := 0, Suc hp := sh sp, Suc (Suc hp) := pc'))) e 
         (vs(vp := hp)) (assm_stk cd sh) nmem nmem) (case_register (3 + hp) ep (Suc vp) (Suc sp) 0 0) 
@@ -395,31 +438,41 @@ next
   thus ?case by auto
 next
   case (evu_apply cd pc h vs vp hp e ep sh sp)
-  moreover from evu_apply have "assemble_code cd ! (16 + assembly_map cd pc) = APop Vals" by simp
-  moreover from evu_apply have "assemble_code cd ! (15 + assembly_map cd pc) = APush Env (Reg Acc)" 
+  moreover from evu_apply have "assemble_code cd ! (23 + assembly_map cd pc) = ASub Vals 1" by simp
+  moreover from evu_apply have "assemble_code cd ! (22 + assembly_map cd pc) = AGet Acc Vals Vals" 
     by simp
-  moreover from evu_apply have "assemble_code cd ! (14 + assembly_map cd pc) = AMov Acc PC" by simp
-  moreover from evu_apply have "assemble_code cd ! (13 + assembly_map cd pc) = ASub Acc 14" by simp
-  moreover from evu_apply have "assemble_code cd ! (12 + assembly_map cd pc) = APush Stk (Reg Acc)" 
+  moreover from evu_apply have "assemble_code cd ! (21 + assembly_map cd pc) = 
+    APut Env Env (Reg Acc)" by simp
+  moreover from evu_apply have "assemble_code cd ! (20 + assembly_map cd pc) = AAdd Env 1" by simp
+  moreover from evu_apply have "assemble_code cd ! (19 + assembly_map cd pc) = AMov Acc PC" by simp
+  moreover from evu_apply have "assemble_code cd ! (18 + assembly_map cd pc) = ASub Acc 19" by simp
+  moreover from evu_apply have "assemble_code cd ! (17 + assembly_map cd pc) = 
+    APut Stk Stk (Reg Acc)" by simp
+  moreover from evu_apply have "assemble_code cd ! (16 + assembly_map cd pc) = AAdd Stk 1" by simp
+  moreover from evu_apply have "assemble_code cd ! (15 + assembly_map cd pc) = AMov Acc (Reg Env)" 
     by simp
-  moreover from evu_apply have "assemble_code cd ! (11 + assembly_map cd pc) = AMov Acc (Reg Env)" 
+  moreover from evu_apply have "assemble_code cd ! (14 + assembly_map cd pc) = AAdd Acc 1" by simp
+  moreover from evu_apply have "assemble_code cd ! (13 + assembly_map cd pc) = 
+    APut Stk Stk (Reg Acc)" by simp
+  moreover from evu_apply have "assemble_code cd ! (12 + assembly_map cd pc) = AAdd Stk 1" by simp
+  moreover from evu_apply have "assemble_code cd ! (11 + assembly_map cd pc) = ASub Vals 1" by simp
+  moreover from evu_apply have "assemble_code cd ! (10 + assembly_map cd pc) = AGet Acc Vals Vals" 
     by simp
-  moreover from evu_apply have "assemble_code cd ! (10 + assembly_map cd pc) = AAdd Acc 1" by simp
-  moreover from evu_apply have "assemble_code cd ! (9 + assembly_map cd pc) = APush Stk (Reg Acc)" 
+  moreover from evu_apply have "assemble_code cd ! (9 + assembly_map cd pc) = AAdd Acc 1" by simp
+  moreover from evu_apply have "assemble_code cd ! (8 + assembly_map cd pc) = AMov Acc2 (Reg Acc)" 
     by simp
-  moreover from evu_apply have "assemble_code cd ! (8 + assembly_map cd pc) = APop Vals" by simp
-  moreover from evu_apply have "assemble_code cd ! (7 + assembly_map cd pc) = AAdd Acc 1" by simp
-  moreover from evu_apply have "assemble_code cd ! (6 + assembly_map cd pc) = AMov Acc2 (Reg Acc)" 
+  moreover from evu_apply have "assemble_code cd ! (7 + assembly_map cd pc) = AGet Acc Hp Acc" 
     by simp
-  moreover from evu_apply have "assemble_code cd ! (5 + assembly_map cd pc) = AGet Hp Acc" 
+  moreover from evu_apply have "assemble_code cd ! (6 + assembly_map cd pc) = 
+    APut Env Env (Reg Acc)" by simp
+  moreover from evu_apply have "assemble_code cd ! (5 + assembly_map cd pc) = AAdd Env 1" by simp
+  moreover from evu_apply have "assemble_code cd ! (4 + assembly_map cd pc) = AMov Acc (Reg Acc2)" 
     by simp
-  moreover from evu_apply have "assemble_code cd ! (4 + assembly_map cd pc) = APush Env (Reg Acc)" 
-    by simp
-  moreover from evu_apply have "assemble_code cd ! (3 + assembly_map cd pc) = AMov Acc (Reg Acc2)" 
+  moreover from evu_apply have "assemble_code cd ! (3 + assembly_map cd pc) = AMov Acc2 (Con 0)" 
     by simp
   moreover from evu_apply have "assemble_code cd ! (2 + assembly_map cd pc) = AAdd Acc 1" 
     by (simp del: add_2_eq_Suc)
-  ultimately have "iter_evala (assemble_code cd) 17 (AS (case_register (assm_hp cd h) e vs 
+  ultimately have "iter_evala (assemble_code cd) 24 (AS (case_register (assm_hp cd h) e vs 
     (assm_stk cd sh) nmem nmem) (case_register hp ep (Suc (Suc vp)) (Suc sp) 0 0) 
       (assembly_map cd (Suc pc))) = Some (AS (case_register (assm_hp cd h) 
         (e(ep := vs (Suc vp), Suc ep := h (Suc (vs vp)))) vs (assm_stk cd (sh(Suc sp := pc, 
@@ -429,9 +482,12 @@ next
   thus ?case by auto
 next
   case (evu_return cd pc h hp e ep vs vp sh sp)
-  moreover from evu_return have "assemble_code cd ! (2 + assembly_map cd pc) = APop Stk" 
+  moreover from evu_return have "assemble_code cd ! (4 + assembly_map cd pc) = ASub Stk 1" by simp
+  moreover from evu_return have "assemble_code cd ! (3 + assembly_map cd pc) = AGet Acc Stk Stk" 
+    by simp
+  moreover from evu_return have "assemble_code cd ! (2 + assembly_map cd pc) = ASub Stk 1" 
     by (simp del: add_2_eq_Suc)
-  ultimately have "iter_evala (assemble_code cd) 3 (AS (case_register (assm_hp cd h) e vs 
+  ultimately have "iter_evala (assemble_code cd) 5 (AS (case_register (assm_hp cd h) e vs 
     (assm_stk cd sh) nmem nmem) (case_register hp ep vp (Suc (Suc sp)) 0 0) 
       (assembly_map cd (Suc pc))) = Some (AS (case_register (assm_hp cd h) e vs (assm_stk cd sh)
         nmem nmem) (case_register hp ep vp sp 0 0) (assembly_map cd (sh sp)))" 
@@ -439,27 +495,39 @@ next
   thus ?case by auto
 next
   case (evu_jump cd pc h vs vp hp e ep sh sp)
-  moreover from evu_jump have "assemble_code cd ! (14 + assembly_map cd pc) = APop Vals" by simp
-  moreover from evu_jump have "assemble_code cd ! (13 + assembly_map cd pc) = APush Env (Reg Acc)" 
+  moreover from evu_jump have "assemble_code cd ! (21 + assembly_map cd pc) = ASub Vals 1" by simp
+  moreover from evu_jump have "assemble_code cd ! (20 + assembly_map cd pc) = AGet Acc Vals Vals" 
     by simp
-  moreover from evu_jump have "assemble_code cd ! (12 + assembly_map cd pc) = APop Stk" by simp
-  moreover from evu_jump have "assemble_code cd ! (11 + assembly_map cd pc) = AMov Acc (Reg Env)" 
+  moreover from evu_jump have "assemble_code cd ! (19 + assembly_map cd pc) = 
+    APut Env Env (Reg Acc)" by simp
+  moreover from evu_jump have "assemble_code cd ! (18 + assembly_map cd pc) = AAdd Env 1" by simp
+  moreover from evu_jump have "assemble_code cd ! (17 + assembly_map cd pc) = ASub Stk 1" by simp
+  moreover from evu_jump have "assemble_code cd ! (16 + assembly_map cd pc) = AGet Acc Stk Stk" 
     by simp
-  moreover from evu_jump have "assemble_code cd ! (10 + assembly_map cd pc) = AAdd Acc 1" by simp
-  moreover from evu_jump have "assemble_code cd ! (9 + assembly_map cd pc) = APush Stk (Reg Acc)" 
+  moreover from evu_jump have "assemble_code cd ! (15 + assembly_map cd pc) = AMov Acc (Reg Env)" 
     by simp
-  moreover from evu_jump have "assemble_code cd ! (8 + assembly_map cd pc) = APop Vals" by simp
-  moreover from evu_jump have "assemble_code cd ! (7 + assembly_map cd pc) = AAdd Acc 1" by simp
-  moreover from evu_jump have "assemble_code cd ! (6 + assembly_map cd pc) = AMov Acc2 (Reg Acc)" 
+  moreover from evu_jump have "assemble_code cd ! (14 + assembly_map cd pc) = AAdd Acc 1" by simp
+  moreover from evu_jump have "assemble_code cd ! (13 + assembly_map cd pc) = APut Stk Stk (Reg Acc)" 
     by simp
-  moreover from evu_jump have "assemble_code cd ! (5 + assembly_map cd pc) = AGet Hp Acc" by simp
-  moreover from evu_jump have "assemble_code cd ! (4 + assembly_map cd pc) = APush Env (Reg Acc)" 
+  moreover from evu_jump have "assemble_code cd ! (12 + assembly_map cd pc) = AAdd Stk 1" by simp
+  moreover from evu_jump have "assemble_code cd ! (11 + assembly_map cd pc) = ASub Vals 1" by simp
+  moreover from evu_jump have "assemble_code cd ! (10 + assembly_map cd pc) = AGet Acc Vals Vals" 
     by simp
-  moreover from evu_jump have "assemble_code cd ! (3 + assembly_map cd pc) = AMov Acc (Reg Acc2)" 
+  moreover from evu_jump have "assemble_code cd ! (9 + assembly_map cd pc) = AAdd Acc 1" by simp
+  moreover from evu_jump have "assemble_code cd ! (8 + assembly_map cd pc) = AMov Acc2 (Reg Acc)" 
+    by simp
+  moreover from evu_jump have "assemble_code cd ! (7 + assembly_map cd pc) = AGet Acc Hp Acc" 
+    by simp
+  moreover from evu_jump have "assemble_code cd ! (6 + assembly_map cd pc) = APut Env Env (Reg Acc)" 
+    by simp
+  moreover from evu_jump have "assemble_code cd ! (5 + assembly_map cd pc) = AAdd Env 1" by simp
+  moreover from evu_jump have "assemble_code cd ! (4 + assembly_map cd pc) = AMov Acc (Reg Acc2)" 
+    by simp
+  moreover from evu_jump have "assemble_code cd ! (3 + assembly_map cd pc) = AMov Acc2 (Con 0)" 
     by simp
   moreover from evu_jump have "assemble_code cd ! (2 + assembly_map cd pc) = AAdd Acc 1" 
     by (simp del: add_2_eq_Suc)
-  ultimately have "iter_evala (assemble_code cd) 15 (AS (case_register (assm_hp cd h) e vs 
+  ultimately have "iter_evala (assemble_code cd) 22 (AS (case_register (assm_hp cd h) e vs 
     (assm_stk cd sh) nmem nmem) (case_register hp ep (Suc (Suc vp)) (Suc sp) 0 0) 
       (assembly_map cd (Suc pc))) = Some (AS (case_register (assm_hp cd h) 
         (e(ep := vs (Suc vp), Suc ep := h (Suc (vs vp)))) vs (assm_stk cd (sh(sp := Suc (Suc ep)))) 
